

$$7. \int (3x+4) \ln(x) dx = \left(\frac{3}{2}x^2 + 4x\right) \ln x - \int \left(\frac{3}{2}x^2 + 4x\right) \frac{1}{x} dx$$

$$\boxed{\begin{array}{ll} u = \ln x & dv = (3x+4)dx \\ du = \frac{1}{x} dx & v = \frac{3}{2}x^2 + 4x \end{array}}$$

$$= \frac{3}{2}x^2 \ln x + 4x \ln x - \int \frac{3}{2}x + 4 dx$$

$$= \frac{3}{2}x^2 \ln x + 4x \ln x - \frac{3}{4}x^2 - 4x + C$$

$$8. \int 3x^2 \sin\left(\frac{1}{5}x\right) dx \quad \text{Tabular}$$

$+ 3x^2$	$\sin\left(\frac{1}{5}x\right)$
$- 6x$	$- 5 \cos\left(\frac{1}{5}x\right)$
$+ 6$	$- 25 \sin\left(\frac{1}{5}x\right)$
$0$	$+ 125 \cos\left(\frac{1}{5}x\right)$

$$- 15x^2 \cos\left(\frac{1}{5}x\right) + 150x \sin\left(\frac{1}{5}x\right) + 750 \cos\left(\frac{1}{5}x\right) + C$$

## 7.2 Trig Integrals

Our two main tools in this section are  $u$ -substitution and trig identities.

### 1 Integrals of the form $\int \sin^m x \cos^n x dx$

#### 1.0.1 Starter Example:

Suppose we want to integrate  $\int \sin^2 x \cos x dx$ . We can do this with  $u$ -substitution.

$$\boxed{\begin{array}{l} u = \sin x \\ du = \cos x dx \end{array}}$$

$$= \int u^2 du = \frac{1}{3} u^3 + C$$

$$= \boxed{\frac{1}{3} \sin^3 x + C}$$

#### 1.1 At least one exponent is odd

Suppose that cosine has an odd exponent. Then let  $u = \sin x$ ,  $du = \cos x dx$ , and use  $\sin^2 x + \cos^2 x = 1$  to rewrite everything in terms of  $\sin x$ .

##### 1.1.1 Example:

$$\int \sin^3 x \cos^4 x dx = \int \sin^2 x \cos^4 x (\sin x dx) = \int (1 - \cos^2 x) \cos^4 x (\sin x dx)$$

$$\boxed{\begin{array}{l} u = \cos x \\ du = -\sin x dx \end{array}}$$

$$= \int (1 - u^2) u^4 (-du) = \int -u^4 + u^6 du$$

$$= -\frac{1}{5} u^5 + \frac{1}{7} u^7 + C$$

$$= \boxed{-\frac{1}{5} \cos^5 x + \frac{1}{7} \cos^7 x + C}$$

### 1.1.2 Example:

$$\int \sin^7 x \cos^5 x \, dx = \int \sin^6 x \cos^4 x (\cos x \, dx)$$

$u = \sin x$   
 $du = \cos x \, dx$

$\uparrow$   
 $(\cos^2 x)^2$   
 $(1 - \sin^2 x)^2$

**Tip:** If both exponents are odd, letting  $u$  be the function with the higher exponent will make for less work.

$$= \int \sin^6 x (1 - \sin^2 x)^2 \cdot (du) = \int u^6 (1 - u^2)^2 \, du$$

$$= \int u^6 (1 - 2u^2 + u^4) \, du = \int u^6 - 2u^8 + u^{10} \, du$$

$$= \frac{1}{7} \sin^7 x - \frac{2}{9} \sin^9 x + \frac{1}{11} \sin^{11} x + C$$

## 1.2 Both exponents are even

If both exponents are even, we rewrite the integral using the double-angle formulas

$$\sin^2 x = \frac{1}{2} [1 - \cos(2x)] \quad \text{and} \quad \cos^2 x = \frac{1}{2} [1 + \cos(2x)]$$